src/HOL/CVC/cvc5_dsl_rewrites/BV_Rewrites_Simplification.thy
@@ -1,0 +1,1748 @@
+theory BV_Rewrites_Simplification
+  imports BV_Rewrites_Lemmas 
+begin
+
+(*Status May 2025: 70 rules total*)
+
+(*
+(define-rule bv-ite-equal-children ((c (_ BitVec 1)) (x ?BitVec)) (bvite c x x) x)
+*)
+
+named_theorems rewrite_bv_ite_equal_children \<open>automatically_generated\<close>
+
+lemma [rewrite_bv_ite_equal_children]:
+  fixes c::"1 word" and x::"'a ::len word"
+  shows "NO_MATCH cvc_a (undefined c x)
+    \<Longrightarrow> (if bit c (0::nat) then x else x) = x"
+  by auto
+
+
+(*
+(define-rule bv-ite-const-children-1 (
+    (c (_ BitVec 1))
+  )
+  (bvite c (@bv 0 1) (@bv 1 1))
+  (bvnot c))
+*)
+
+named_theorems rewrite_bv_ite_const_children_1 \<open>automatically_generated\<close>
+
+lemma [rewrite_bv_ite_const_children_1]:
+  fixes c::"1 word"
+  shows "NO_MATCH cvc_a (undefined c)
+    \<Longrightarrow> (if bit c (0::nat) then Word.Word (0::int) else Word.Word (1::int)) = not c"
+  by (metis (mono_tags, opaque_lifting) Word.of_nat_unat Word_eq_word_of_int add.group_left_neutral bit.compl_one bit.compl_zero bit_0_eq inc_le len_of_numeral_defs(2) mask_1 nat_int nle_le nth_0 take_bit_minus_one_eq_mask test_bit_1 ucast_id unsigned_1 unsigned_of_int word_neq_0_conv word_of_int_0 word_of_int_1 word_of_int_neg_1 word_order.extremum)
+
+
+(*
+(define-rule bv-ite-const-children-2 (
+    (c (_ BitVec 1))
+  )
+  (bvite c (@bv 1 1) (@bv 0 1))
+  c)
+*)
+
+named_theorems rewrite_bv_ite_const_children_2 \<open>automatically_generated\<close>
+
+lemma [rewrite_bv_ite_const_children_2]:
+  fixes c::"1 word"
+  shows "NO_MATCH cvc_a (undefined c)
+    \<Longrightarrow> (if bit c (0::nat) then Word.Word (1::int) else Word.Word (0::int)) = c"
+  by (metis (mono_tags, opaque_lifting) Word.of_nat_unat add.group_left_neutral bit.compl_zero len_of_numeral_defs(2) mask_1 nat_int nth_0 one_word_def take_bit_minus_one_eq_mask ucast_id unsigned_1 unsigned_of_int word_and_1 word_ao_nth word_exists_nth word_of_int_neg_1 word_plus_and_or_coroll2 zero_word_def)
+
+
+(*
+(define-rule bv-ite-equal-cond-1 (
+    (c0 (_ BitVec 1))
+    (t0 ?BitVec)
+    (e0 ?BitVec)
+    (e1 ?BitVec)
+  )
+  (bvite c0 (bvite c0 t0 e0) e1)
+  (bvite c0 t0 e1))
+*)
+
+named_theorems rewrite_bv_ite_equal_cond_1 \<open>automatically_generated\<close>
+
+lemma [rewrite_bv_ite_equal_cond_1]:
+  fixes c0::"1 word" and t0::"'a ::len word" and e0::"'a ::len word" and e1::"'a ::len word"
+  shows "NO_MATCH cvc_a (undefined c0 t0 e0 e1)
+    \<Longrightarrow> (if bit c0 (0::nat) then if bit c0 (0::nat) then t0 else e0 else e1) =
+   (if bit c0 (0::nat) then t0 else e1)"
+  by auto
+
+
+(*
+(define-rule bv-ite-equal-cond-2 (
+    (c0 (_ BitVec 1))
+    (t0 ?BitVec)
+    (t1 ?BitVec)
+    (e1 ?BitVec)
+  )
+  (bvite c0 t0 (bvite c0 t1 e1))
+  (bvite c0 t0 e1))
+*)
+
+named_theorems rewrite_bv_ite_equal_cond_2 \<open>automatically_generated\<close>
+
+lemma [rewrite_bv_ite_equal_cond_2]:
+  fixes c0::"1 word" and t0::"'a ::len word" and t1::"'a ::len word" and e1::"'a ::len word"
+  shows "(if bit c0 (0::nat) then t0 else if bit c0 (0::nat) then t1 else e1) =
+   (if bit c0 (0::nat) then t0 else e1)"
+  by auto
+
+
+(*
+(define-rule bv-ite-equal-cond-3 (
+    (c0 (_ BitVec 1))
+    (t0 ?BitVec)
+    (e0 ?BitVec)
+    (t1 ?BitVec)
+    (e1 ?BitVec)
+  )
+  (bvite c0 (bvite c0 t0 e0) (bvite c0 t1 e1))
+  (bvite c0 t0 e1))
+*)
+
+
+named_theorems rewrite_bv_ite_equal_cond_3 \<open>automatically_generated\<close>
+
+lemma [rewrite_bv_ite_equal_cond_3]:
+  fixes c0::"1 word" and t0::"'a ::len word" and e0::"'a ::len word" and t1::"'a ::len word" and e1::"'a ::len word"
+  shows "(if bit c0 (0::nat) then if bit c0 (0::nat) then t0 else e0
+    else if bit c0 (0::nat) then t1 else e1) =
+   (if bit c0 (0::nat) then t0 else e1)"
+  by auto
+
+(*
+(define-rule bv-ite-merge-then-if (
+    (c0 (_ BitVec 1))
+    (c1 (_ BitVec 1))
+    (t1 ?BitVec)
+    (e1 ?BitVec)
+  )
+  (bvite c0 (bvite c1 t1 e1) t1)
+  (bvite (bvand c0 (bvnot c1)) e1 t1))
+*)
+
+named_theorems rewrite_bv_ite_merge_then_if \<open>automatically_generated\<close>
+
+lemma [rewrite_bv_ite_merge_then_if]:
+  fixes c0::"1 word" and c1::"1  word" and t1::"'a ::len word" and e1::"'a ::len word"
+  shows "(if bit c0 (0::nat) then if bit c1 (0::nat) then t1 else e1 else t1) =
+   (if bit (and c0 (not c1)) (0::nat) then e1 else t1)"
+  by (metis lsb0)
+
+
+(*
+(define-rule bv-ite-merge-else-if (
+    (c0 (_ BitVec 1))
+    (c1 (_ BitVec 1))
+    (t1 ?BitVec)
+    (e1 ?BitVec)
+  )
+  (bvite c0 (bvite c1 t1 e1) e1)
+  (bvite (bvand c0 c1) t1 e1))
+*)
+
+named_theorems rewrite_bv_ite_merge_else_if \<open>automatically_generated\<close>
+
+lemma [rewrite_bv_ite_merge_else_if]:
+  fixes c0::"1 word" and c1::"1 word" and t1::"'a ::len word" and e1::"'a ::len word"
+  shows "(if bit c0 (0::nat) then if bit c1 (0::nat) then t1 else e1 else e1) =
+   (if bit (and c0 c1) (0::nat) then t1 else e1)"
+  by (metis word_ao_nth)
+
+
+(*
+(define-rule bv-ite-merge-then-else (
+    (c0 (_ BitVec 1))
+    (c1 (_ BitVec 1))
+    (t0 ?BitVec)
+    (e1 ?BitVec)
+  )
+  (bvite c0 t0 (bvite c1 t0 e1))
+  (bvite (bvand (bvnot c0) (bvnot c1)) e1 t0))
+*)
+
+named_theorems rewrite_bv_ite_merge_then_else \<open>automatically_generated\<close>
+
+lemma [rewrite_bv_ite_merge_then_else]:
+  fixes c0::"1 word" and c1::"1 word" and t0::"'a ::len word" and e1::"'a ::len word"
+  shows "(if bit c0 (0::nat) then t0 else if bit c1 (0::nat) then t0 else e1) =
+   (if bit (not (or c0 c1)) (0::nat) then e1 else t0)"
+  by (metis lsb0)
+
+
+(*
+(define-rule bv-ite-merge-else-else (
+    (c0 (_ BitVec 1))
+    (c1 (_ BitVec 1))
+    (t1 ?BitVec)
+    (t0 ?BitVec)
+  )
+  (bvite c0 t0 (bvite c1 t1 t0))
+  (bvite (bvand (bvnot c0) c1) t1 t0))
+*)
+
+named_theorems rewrite_bv_ite_merge_else_else \<open>automatically_generated\<close>
+
+lemma [rewrite_bv_ite_merge_else_else]:
+  fixes c0::"1  word" and c1::"1 word" and t1::"'a ::len word" and t0::"'a ::len word"
+  shows "(if bit c0 (0::nat) then t0 else if bit c1 (0::nat) then t1 else t0) =
+   (if bit (and (not c0) c1) (0::nat) then t1 else t0)"
+  by (metis lsb0)
+
+
+(*
+(define-rule bv-shl-by-const-0
+  ((x ?BitVec) (sz Int))
+  (bvshl x (@bv 0 sz))
+  x)
+*)
+
+named_theorems rewrite_bv_shl_by_const_0 \<open>automatically_generated\<close>
+
+lemma [rewrite_bv_shl_by_const_0]:
+  fixes x::"'a::len word" and sz::"int"
+  shows "push_bit (unat (Word.Word (0::int))) x = x"
+  by auto
+
+
+(*
+(define-cond-rule bv-shl-by-const-1
+  ((x ?BitVec) (amount Int) (sz Int) (en Int))
+  (def (n (@bvsize x)))
+  (and (< amount n) (= en (- n (+ 1 amount))))
+  (bvshl x (@bv amount sz))
+  (concat (extract en 0 x) (@bv 0 amount)))
+*)
+
+named_theorems rewrite_bv_shl_by_const_1 \<open>automatically_generated\<close>
+
+lemma [rewrite_bv_shl_by_const_1]:
+  fixes x::"'a::len word" and amount::"int" and sz::"int" and en::"int"
+  shows "NO_MATCH cvc_a (undefined x amount sz en)
+    \<Longrightarrow> (amount < int(size x)) = True
+    \<Longrightarrow> en = int (size x) - (1 + amount)
+    \<Longrightarrow> LENGTH('b) = amount \<Longrightarrow> LENGTH('a) = LENGTH('c) + LENGTH('b) \<Longrightarrow> LENGTH('c) = en + 1
+    \<Longrightarrow>
+   (push_bit (nat amount) x ::'a::len word)=
+   word_cat
+    (smt_extract (nat en) (nat (0::int)) x::'c::len word)
+    (0::'b::len word)"
+  apply (subst word_unat_eq_iff)
+  apply (simp only: unsigned_push_bit_eq unat_word_cat)
+  apply (subst unat_smt_extract)
+     apply simp_all
+  apply (simp only: take_bit_push_bit)
+  apply (rule arg_cong2[where f = push_bit])
+   apply simp
+  apply (rule arg_cong2[where f = take_bit])
+   apply simp
+  apply simp
+  done
+
+(*
+(define-cond-rule bv-shl-by-const-2
+  ((x ?BitVec) (amount Int) (sz Int) (w Int))
+  (and (>= amount (@bvsize x)) (= w (@bvsize x)))
+  (bvshl x (@bv amount sz))
+  (@bv 0 w))
+*)
+
+named_theorems rewrite_bv_shl_by_const_2 \<open>automatically_generated\<close>
+
+lemma [rewrite_bv_shl_by_const_2]:
+  fixes x::"'a ::len word" and amount::"int" and sz::"int"
+  shows "int (size x) \<le> amount \<longrightarrow> LENGTH('b) = sz \<longrightarrow> amount < 2^LENGTH('b) \<longrightarrow>
+   push_bit (unat (Word.Word amount::'b::len word)) x = (Word.Word (0::int)::'a::len word)"
+  by (simp add: take_bit_int_eq_self unsigned_of_int word_size)
+
+
+(*
+(define-rule bv-lshr-by-const-0
+  ((x ?BitVec) (sz Int))
+  (bvlshr x (@bv 0 sz))
+  x)
+*)
+
+named_theorems rewrite_bv_lshr_by_const_0 \<open>automatically_generated\<close>
+
+lemma [rewrite_bv_lshr_by_const_0]:
+  fixes x::"'a ::len word"  and sz::"int"
+  shows "LENGTH('b) = sz \<longrightarrow>
+   drop_bit (unat (Word.Word 0::'b::len word)) x = x"
+  by force
+
+
+(*
+(define-cond-rule bv-lshr-by-const-1
+  ((x ?BitVec) (amount Int) (sz Int) (nm1 Int))
+  (def (n (@bvsize x)))
+  (and (< amount n) (= nm1 (- n 1)))
+  (bvlshr x (@bv amount sz))
+  (concat (@bv 0 amount) (extract nm1 amount x)))
+*)
+
+named_theorems rewrite_bv_lshr_by_const_1 \<open>automatically_generated\<close>
+
+lemma [rewrite_bv_lshr_by_const_1]:
+  fixes x::"'a ::len word" and amount::"int" and sz::"int"
+  shows "amount < int (size x) \<longrightarrow>
+   LENGTH('a) = LENGTH('b) + LENGTH('c) \<longrightarrow>
+  (nat (int (size x) - (1::int))) < LENGTH('a) \<longrightarrow>
+  0 \<le> amount \<longrightarrow>
+(nat amount) \<le> (nat (int (size x) - (1::int))) \<longrightarrow>
+  LENGTH('c) = 1 + ((nat (int (size x) - (1::int))) - (nat amount)) \<longrightarrow>
+amount < 2^LENGTH('d) \<longrightarrow>
+LENGTH('d) = sz \<longrightarrow>
+   (drop_bit (unat (Word.Word amount::'d::len word)) x::'a::len word) =
+   word_cat (Word.Word (0::int)::'b::len word)
+    (smt_extract (nat (int (size x) - (1::int))) (nat amount) x::'c::len word)"
+  apply rule+
+proof-
+  assume a0: "amount < int (size x)"
+    "LENGTH('a) = LENGTH('b) + LENGTH('c)"
+    "nat (int (size x) - (1::int)) < LENGTH('a)"
+    "(0::int) \<le> amount"
+    "nat amount \<le> nat (int (size x) - (1::int))"
+    "LENGTH('c) = (1::nat) + (nat (int (size x) - (1::int)) - nat amount)"
+    "amount < (2::int) ^ LENGTH('d)"
+    "int LENGTH('d) = sz"
+  have t0: "min (LENGTH('c::len) + nat amount) LENGTH('a) = LENGTH('a)"
+    by (smt (verit, ccfv_SIG) a0(5) a0(6) add_diff_cancel_left' diff_add diff_diff_left less_le_not_le min.commute min.idem min.order_iff nat_minus_as_int nat_neq_iff of_nat_1 word_size)
+   have t1: "(take_bit LENGTH('d) amount) = amount"
+    apply (subst take_bit_int_eq_self[of amount "LENGTH('d)" ])
+    apply (simp add: a0)
+    using a0(7) apply auto[1]
+    by auto
+
+  have "(word_cat (Word.Word (0::int)::'b::len word)
+    (smt_extract (nat (int (size x) - (1::int))) (nat amount) x::'c::len word)::'a::len word)
+  = word_cat (0::'b::len word)
+    (smt_extract (size x - 1) (nat amount) x::'c::len word)"
+    by (metis nat_minus_as_int of_nat_1 zero_word_def)
+  also have "...
+  = word_cat (0::'b word) (slice (nat amount) (take_bit (size x) x)::'c::len word)"
+    unfolding smt_extract_def
+    by simp
+  also have "...
+  = word_cat (0::'b word) (slice (nat amount) x::'c::len word)"
+    using take_bit_length_eq
+    by (simp add: word_size)
+  also have "...
+  = word_cat (0::'b word) (slice1 (LENGTH('a::len) - nat amount) x::'c::len word)"
+    using slice_def[of "nat amount"]
+    by (simp add: slice_def)
+ also have "...
+  = word_cat (0::'b word) (ucast (drop_bit (LENGTH('a::len) - (LENGTH('a::len) - nat amount)) x)::'c::len word)"
+   using slice1_def[of "(LENGTH('a::len) - nat amount)" x]
+   by (smt (verit, del_insts) One_nat_def Suc_diff_1 a0(2) a0(5) a0(6) diff_add_inverse diff_less_mono2 len_gt_0 nat_diff_distrib' nat_int nat_one_as_int of_nat_0_le_iff ordered_cancel_comm_monoid_diff_class.add_diff_assoc plus_1_eq_Suc size_word.rep_eq)
+ also have "...
+  = word_cat (0::'b word) (ucast (drop_bit (nat amount) x)::'c::len word)"
+   by (metis a0(1) diff_diff_cancel less_le_not_le nat_le_iff word_size)
+ also have "...
+  =  push_bit LENGTH('c::len) (ucast (0::'b word)) + ucast (ucast (drop_bit (nat amount) x)::'c::len word)"
+   using word_cat_eq
+   by blast
+also have "...
+  =  push_bit LENGTH('c::len) 0 + ucast (ucast (drop_bit (nat amount) x)::'c::len word)"
+  using unsigned_ucast_eq[of "(drop_bit (nat amount) x)"]
+  by auto
+also have "...
+  = ucast (ucast (drop_bit (nat amount) x)::'c::len word)"
+  by simp
+also have "...
+  = (take_bit LENGTH('c::len) (unsigned (drop_bit (nat amount) x)::'a::len word))"
+  using unsigned_ucast_eq[of "(drop_bit (nat amount) x)"]
+  by (smt (verit, del_insts))
+also have "...
+  = (take_bit LENGTH('c::len) (drop_bit (nat amount) (take_bit LENGTH('a::len) (unsigned x))))"
+  using unsigned_drop_bit_eq[of "nat amount" x] by simp
+also have "...
+  = drop_bit (nat amount) (take_bit (LENGTH('c::len) + nat amount) (take_bit LENGTH('a::len) (unsigned x)))"
+  using take_bit_drop_bit[of "LENGTH('c)" "nat amount" "(take_bit LENGTH('a::len) (unsigned x))"]
+  by blast
+also have "...
+  = drop_bit (nat amount) (take_bit LENGTH('a::len) (unsigned x))"
+  using take_bit_take_bit
+  by (smt (verit, ccfv_threshold) One_nat_def Suc_pred a0(5) a0(6) diff_add group_cancel.add1 int_ops(2) len_gt_0 nat_int_comparison(3) nat_minus_as_int plus_1_eq_Suc size_word.rep_eq take_bit_word_beyond_length_eq)
+also have "...
+  = drop_bit (nat amount) (unsigned x)"
+  by force
+  finally have "(word_cat (Word.Word (0::int)::'b::len word)
+    (smt_extract (nat (int (size x) - (1::int))) (nat amount) x::'c::len word)::'a::len word)
+  = drop_bit (nat amount) (unsigned x)"
+    by blast
+
+    then show "(drop_bit (unat (Word.Word amount::'d::len word)) x::'a::len word) =
+   word_cat (Word.Word (0::int)::'b::len word)
+    (smt_extract (nat (int (size x) - (1::int))) (nat amount) x::'c::len word)"
+            by (simp add: a0(4) a0(7) unat_eq_nat_uint word_of_int_inverse)
+        qed
+
+
+(*
+(define-cond-rule bv-lshr-by-const-2
+  ((x ?BitVec) (amount Int) (sz Int))
+  (>= amount (@bvsize x))
+  (bvlshr x (@bv amount sz))
+  (@bv 0 sz))
+*)
+
+
+(*
+(define-rule bv-ashr-by-const-0
+  ((x ?BitVec) (sz Int))
+  (bvashr x (@bv 0 sz))
+  x)
+*)
+
+
+(*
+(define-cond-rule bv-ashr-by-const-1
+  ((x ?BitVec) (amount Int) (sz Int) (nm1 Int))
+  (def (n (@bvsize x)))
+  (and (< amount n) (= nm1 (- n 1)))
+  (bvashr x (@bv amount sz))
+  (concat
+    (repeat amount (extract nm1 nm1 x))
+    (extract nm1 amount x)
+  ))
+*)
+
+
+(*
+(define-cond-rule bv-ashr-by-const-2
+  ((x ?BitVec) (amount Int) (sz Int) (nm1 Int) (rn Int))
+  (and (>= amount (@bvsize x)) (= nm1 (- (@bvsize x) 1)) (= rn (@bvsize x)))
+  (bvashr x (@bv amount sz))
+  (repeat rn (extract nm1 nm1 x)))
+*)
+
+
+
+(*
+(define-cond-rule bv-and-concat-pullup
+  ((xs ?BitVec :list) (ws ?BitVec :list) (y ?BitVec)
+   (z ?BitVec) (ys ?BitVec :list)
+   (nxm1 Int) (ny Int) (nym1 Int))
+  (def
+    (nx (@bvsize (bvand xs ws)))
+  )
+  (and (= ny (@bvsize y)) (= nxm1 (- nx 1)) (= nym1 (- (@bvsize y) 1)))
+  (bvand xs (concat ys z y) ws)
+  (concat
+    (bvand (extract nxm1 ny (bvand xs ws)) (concat ys z))
+    (bvand (extract nym1 0 (bvand xs ws)) y)
+  ))
+*)
+
+(*
+(define-cond-rule bv-or-concat-pullup
+  ((xs ?BitVec :list) (ws ?BitVec :list) (y ?BitVec)
+   (z ?BitVec) (ys ?BitVec :list)
+   (nxm1 Int) (ny Int) (nym1 Int))
+  (def
+    (nx (@bvsize (bvor xs ws)))
+  )
+  (and (= ny (@bvsize y)) (= nxm1 (- nx 1)) (= nym1 (- (@bvsize y) 1)))
+  (bvor xs (concat ys z y) ws)
+  (concat
+    (bvor (extract nxm1 ny (bvor xs ws)) (concat ys z))
+    (bvor (extract nym1 0 (bvor xs ws)) y)
+  ))
+*)
+
+(*
+(define-cond-rule bv-xor-concat-pullup
+  ((xs ?BitVec :list) (ws ?BitVec :list) (y ?BitVec)
+   (z ?BitVec) (ys ?BitVec :list)
+   (nxm1 Int) (ny Int) (nym1 Int))
+  (def
+    (nx (@bvsize (bvxor xs ws)))
+  )
+  (and (= ny (@bvsize y)) (= nxm1 (- nx 1)) (= nym1 (- (@bvsize y) 1)))
+  (bvxor xs (concat ys z y) ws)
+  (concat
+    (bvxor (extract nxm1 ny (bvxor xs ws)) (concat ys z))
+    (bvxor (extract nym1 0 (bvxor xs ws)) y)
+  ))
+*)
+named_theorems rewrite_bv_xor_concat_pullup \<open>automatically_generated\<close>
+
+fun word_cat_rbl_left :: "bool list list \<Rightarrow> 'a ::len word \<Rightarrow> 'b::len  word" where
+  "word_cat_rbl_left xs y = word_cat (of_bl (concat xs)::'b:: len word) y"
+
+lemma bit_foldr_xor:
+"bit (foldr xor xs y) n = foldr (\<noteq>) (map (\<lambda>x. bit x n) xs) (bit y n)"
+  apply (induction xs)
+   apply simp_all
+  by (simp add: bit_xor_iff)
+
+fun is_singleton_ListVar:: "'a cvc_ListVar \<Rightarrow> bool" where
+ "is_singleton_ListVar (ListVar xs) = (length xs = 1)"
+fun is_empty_ListVar:: "'a cvc_ListVar \<Rightarrow> bool" where
+ "is_empty_ListVar (ListVar xs) = (length xs = 0)"
+
+
+fun word_cat_helper_left::"('a::len word) cvc_ListVar \<Rightarrow> 'b::len word \<Rightarrow> 'c::len word" where
+"word_cat_helper_left (ListVar [x]) y = (word_cat x y)"
+
+fun word_cat_helper_empty_left::"('a::len word) cvc_ListVar \<Rightarrow> 'b::len word \<Rightarrow> 'b::len word" where
+"word_cat_helper_empty_left (ListVar []) y = y"
+
+
+lemmas word_cat_helper_def = word_cat_helper_left.simps word_cat_helper_empty_left.simps
+
+lemma helper:
+"n \<le> size y \<Longrightarrow> bit (xor xs (word_cat x y)) n = bit (xor xs y) n"
+  unfolding bit_xor_iff bit_word_cat_iff
+  by (simp add: word_size)
+
+lemma helper3:
+" (xor x (foldr xor xs y)) = (foldr xor (x # xs) y)"
+  by simp
+
+lemma helper3b:
+" (xor (foldr xor xs y) x) = (foldr xor (xs @ [y]) x)"
+  apply (induction xs)
+   apply simp_all
+  
+  by (simp add: xor.assoc)
+
+
+lemma helper4:
+" (foldr xor xs (foldr xor ys y)) = (foldr xor (xs @ ys) y)"
+  by simp
+
+lemma helper5:
+"(0::int) \<le> m \<Longrightarrow>  m \<le> n \<Longrightarrow> nat n < LENGTH('b) \<Longrightarrow> int LENGTH('a) = n + (1::int) - m \<Longrightarrow>
+ (smt_extract (nat n) (nat m) (foldr xor xs (y::'b::len word)::'b ::len word)::'a::len word) = foldr xor (map (smt_extract (nat n) (nat m)) xs) (smt_extract (nat n) (nat m) y)"
+  apply (induction xs)
+  apply simp_all
+  apply (subst rewrite_bv_extract_bitwise_xor)
+      apply (simp_all add: word_size)
+  done
+
+lemma helper6: 
+" (0::nat) = nat (0::int)"
+  by simp
+
+
+
+lemma case1: 
+ fixes xs::"('a::len word) list"
+    and x::"('a::len word)"
+    and y::"'b::len word"
+    and z::"'c::len word"
+    and n::"nat"
+  assumes "n < LENGTH('b)" and  "n < LENGTH('a)"
+  shows "bit ((xor (word_cat z y::'a::len word) x)) n = 
+bit (xor (smt_extract n 0 y ::'a::len word) (smt_extract n 0 x)) n"
+  apply (simp add: bit_xor_iff bit_smt_extract)
+  by (simp_all add: bit_word_cat_iff assms)
+
+lemma yip1: "slice n (xor a b) = (xor (slice n a) (slice n b))"
+  unfolding slice_def slice1_def
+  by (simp add: unsigned_xor_eq)
+
+lemma yip2: "
+ smt_extract n (0::nat) (foldr xor xs y) = foldr xor (map (smt_extract n  (0::nat)) xs) (smt_extract n (0::nat) y) "
+  apply (induction xs)
+   apply simp_all
+  unfolding smt_extract_def
+  subgoal for x xss
+    apply (subst take_bit_xor[of "(Suc n)" x])
+    apply (subst yip1)
+    by presburger
+  done
+
+lemma yip3:
+"n < LENGTH('a::len) \<Longrightarrow> LENGTH('a)  < LENGTH('b) \<Longrightarrow>
+(map ((\<lambda>x::'b ::len word. bit x n) \<circ> smt_extract (LENGTH('a) - Suc (0::nat)) (0::nat)) xs') = (map ((\<lambda>x::'b word. bit x n)) (xs'::'b::len word list))"
+  apply (induction xs')
+   apply simp_all
+  unfolding bit_smt_extract
+  by simp_all
+
+lemma yip4:
+"n < LENGTH('a::len) \<Longrightarrow> LENGTH('a) < LENGTH('b::len) \<Longrightarrow> (map (smt_extract (LENGTH('a)) 0) (x#xs)) = y#ys 
+\<Longrightarrow> 
+ bit (foldr xor xs (x::'a word)) n = bit (foldr xor ys (y::'b word)) n"
+  apply (induction xs)
+   apply simp_all
+  oops
+
+definition xor_bin where
+ "xor_bin \<equiv> foldr (\<lambda>(x::bool) y::bool. x = (\<not> y))"
+
+
+definition bit_map where
+ "bit_map n \<equiv> map (\<lambda>x::'a ::len word. bit x n) "
+
+lemma smt_extract_over:
+"a - Suc 0< LENGTH('b::len) \<Longrightarrow> n \<le> a -Suc 0 \<Longrightarrow> bit (smt_extract (a-Suc 0) (0::nat) t1::'b::len word) n = bit (t1::'a::len word) n"
+  unfolding smt_extract_def
+  by (simp add: nth_slice bit_take_bit_iff)
+
+lemma smt_extract_shift:
+"n \<ge> LENGTH('b) \<Longrightarrow> n < LENGTH('b) + LENGTH('c) \<Longrightarrow> n - LENGTH('b) < LENGTH('d) \<Longrightarrow> bit (smt_extract (LENGTH('b::len) + LENGTH('c::len) - Suc (0::nat)) LENGTH('b) (t1::'a::len word)::'d::len word ) (n - LENGTH('b))
+= bit t1 n
+"
+  unfolding smt_extract_def
+  by (simp add: nth_slice bit_take_bit_iff)
+
+
+
+
+
+lemma rewrite_bv_xor_concat_pullup_lemma0:
+  fixes t1::"('a::len word) "
+    and t2::"('d::len word)"
+    and y::"'c::len word"
+  shows "LENGTH('a::len) = LENGTH('d) + LENGTH('c)
+\<Longrightarrow>
+   (xor (word_cat t2 y ::'a::len word) t1)
+   =    
+  (word_cat
+    (xor (smt_extract (LENGTH('a) - 1) (LENGTH('c)) t1 ::'d::len word) t2 ::'d::len word)
+    (xor (smt_extract (LENGTH('c) - 1) (nat 0)      t1 ::'c::len word) y  ::'c::len word)
+  ::'a word)
+   "
+  apply (simp add: bang_eq)
+  apply (rule allI)
+  subgoal for n
+    apply (simp add: bit_xor_iff bit_word_cat_iff bit_smt_extract)
+    apply (cases "n < LENGTH('c)")
+     apply simp_all
+     apply blast
+    by (metis add_diff_inverse_nat bit_imp_le_length le_add1 less_diff_conv2)
+  done
+
+lemma rewrite_bv_xor_concat_pullup_lemma1:
+  fixes t1::"('a::len word)"
+    and y::"'b::len word"
+    and z::"'c::len word"
+  shows "LENGTH('a) = LENGTH('b) + LENGTH('c)
+\<Longrightarrow> LENGTH('b) \<ge> 1 \<Longrightarrow> LENGTH('a) \<ge> 1
+\<Longrightarrow>
+   (xor (word_cat z y ::'a ::len word) t1::'a word)
+= 
+  (word_cat
+    (xor (smt_extract ( LENGTH('a) - 1) (LENGTH('b)) (t1 ::'a::len word)::'c::len word) (z::'c::len word) ::'c::len word)
+    (xor (smt_extract (LENGTH('b) - 1)  (nat 0)      (t1 ::'a::len word)::'b::len word) (y::'b::len word) ::'b::len word)
+    ::'a word)
+"
+  using rewrite_bv_xor_concat_pullup_lemma0 
+  by (metis add.commute)
+  
+(*
+(define-cond-rule bv-xor-concat-pullup
+  ((xs ?BitVec :list) (ws ?BitVec :list) (y ?BitVec)
+   (z ?BitVec) (ys ?BitVec :list)
+   )
+  (bvxor xs (concat ys (concat z y)) ws)
+  (concat
+    (bvxor (extract (- (@bvsize (bvxor xs ws)) 1) (@bvsize y) (bvxor xs ws)) (concat ys z))
+    (bvxor (extract (- (@bvsize y) 1) 0 (bvxor xs ws)) y)
+  ))
+
+size xs = size ws = size z + size y
+xs \<rightarrow> 'a word
+ws \<rightarrow> 'a word
+
+z \<longrightarrow> 'c word
+y \<longrightarrow> 'b word
+(concat z y)  \<longrightarrow> 'a word = 'b word + 'c word
+(bvxor xs (concat ys (concat z y)) ws) \<longrightarrow> 'a word
+(@bvsize (bvxor xs ws)) \<longrightarrow> 'a word
+(concat ys z) \<longrightarrow> 'c word
+(extract (- (@bvsize (bvxor xs ws)) 1) (@bvsize y) (bvxor xs ws)) \<longrightarrow> 'c word = ('a word)  - ('b word)
+(extract (- (@bvsize y) 1) 0 (bvxor xs ws)) \<longrightarrow> 'b word
+(concat
+    (bvxor (extract (- (@bvsize (bvxor xs ws)) 1) (@bvsize y) (bvxor xs ws)) (concat ys z))
+    (bvxor (extract (- (@bvsize y) 1) 0 (bvxor xs ws)) y)
+  )) \<longrightarrow> 'a word = 'c word + 'b word
+
+*)
+
+lemma fold_a:"foldr xor (xs' @ ys') x = foldr xor (ys' @ xs') x "
+  apply (induction xs')
+   apply simp_all
+  apply (induction ys')
+   apply simp_all
+  by (metis (mono_tags, opaque_lifting) foldr_append helper3 helper3b xor.commute)
+
+lemma fold_b: "foldr xor (xs' @ word_cat z y # butlast ws') (last ws') = foldr xor (word_cat z y # xs' @ butlast ws') (last ws') "
+  by (metis append_Cons fold_a helper3)
+
+lemma rewrite_bv_xor_concat_pullup_empty:
+  fixes xs::"('a::len word) cvc_ListVar"
+    and ws::"('a::len word) cvc_ListVar"
+    and y::"'b::len word"
+    and z::"'c::len word"
+    and ys::"('e::len word) cvc_ListVar"
+  shows "LENGTH('a) = LENGTH('b) + LENGTH('c)
+\<Longrightarrow> xs \<noteq> (ListVar []) \<Longrightarrow> ws \<noteq> (ListVar []) \<Longrightarrow> is_empty_ListVar ys
+\<Longrightarrow>
+   (cvc_list_left xor xs
+     (cvc_list_right xor
+      (word_cat z y ::'a ::len word)
+       ws
+     ::'a word)
+   ::'a word)
+= 
+  (word_cat
+    ( xor
+      (smt_extract ( LENGTH('a) - 1) (LENGTH('b)) (cvc_list_both' xor xs ws ::'a::len word)::'c::len word)
+      (z::'c::len word)
+    ::'c::len word)
+    (xor (smt_extract (LENGTH('b) - 1) (nat 0) (cvc_list_both' xor xs ws ::'a word)::'b::len word) y ::'b word)
+  ::'a word)
+   "
+apply (cases xs)
+  apply (cases ws)
+  apply (cases ys)
+  apply simp
+  subgoal for xs' ws' ys'
+      unfolding cvc_list_left_transfer
+      apply (subst cvc_list_right_transfer_2)
+       apply simp
+      unfolding cvc_list_both_transfer'
+         apply (simp only: helper3 helper4 helper3b)
+      apply (subst fold_b)
+      apply simp
+      apply (subst rewrite_bv_xor_concat_pullup_lemma1[of z y "(foldr xor xs' (foldr xor (butlast ws') (last ws')))"])
+         apply (simp_all add: le_def)
+      done
+    done
+
+lemma [rewrite_bv_xor_concat_pullup]:
+  fixes xs::"('a::len word) cvc_ListVar"
+    and ws::"('a::len word) cvc_ListVar"
+    and y::"'b::len word"
+    and z::"'c::len word"
+    and ys::"('e::len word) cvc_ListVar"
+    and nxm1::int and ny::int and nym1::int
+shows "NO_MATCH cvc_a (undefined xs ws y z ys nxm1 ny nym1)
+\<Longrightarrow> LENGTH('a) = LENGTH('b) + LENGTH('c)
+\<Longrightarrow> xs \<noteq> (ListVar []) \<Longrightarrow> ws \<noteq> (ListVar []) \<Longrightarrow> is_empty_ListVar ys
+\<Longrightarrow>
+   (cvc_list_left xor xs
+     (cvc_list_right xor
+       (word_cat_helper_empty_left 
+         ys
+         (word_cat z y ::'a ::len word)
+       ::'a::len word)
+       ws
+     ::'a word)
+   ::'a word)
+= 
+  (word_cat
+    ( xor
+      (smt_extract ( LENGTH('a) - 1) (LENGTH('b)) (cvc_list_both' xor xs ws ::'a::len word)::'c::len word)
+      (word_cat_helper_empty_left ys (z::'c::len word)::'c::len word)
+    ::'c::len word)
+    (xor (smt_extract (LENGTH('b) - 1) (nat 0) (cvc_list_both' xor xs ws ::'a word)::'b::len word) y ::'b word)
+  ::'a word)
+   "
+  apply (cases ys)
+  apply simp
+ 
+  using rewrite_bv_xor_concat_pullup_empty[of xs ws ys z y] 
+  by fastforce
+
+
+(*(define-cond-rule bv-xor-concat-pullup
+  ((xs ?BitVec :list) (ws ?BitVec :list) (y ?BitVec)
+   (z ?BitVec) (ys ?BitVec :list)
+   (nxm1 Int) (ny Int) (nym1 Int))
+  (def
+    (nx (@bvsize (bvxor xs ws)))
+  )
+  (and (= ny (@bvsize y)) (= nxm1 (- nx 1)) (= nym1 (- (@bvsize y) 1)))
+  (bvxor xs (concat ys z y) ws)
+  (concat
+    (bvxor (extract nxm1 ny (bvxor xs ws)) (concat ys z))
+    (bvxor (extract nym1 0 (bvxor xs ws)) y)
+  ))*)
+
+lemma [rewrite_bv_xor_concat_pullup]:
+  fixes xs::"('a::len word) cvc_ListVar"
+    and ws::"('a::len word) cvc_ListVar"
+    and y::"'b::len word"
+    and z::"'c::len word"
+    and ys::"('e::len word) cvc_ListVar"
+    and nxm1::int and ny::int and nym1::int
+  shows "NO_MATCH cvc_a (undefined xs ws y z ys nxm1 ny nym1)
+\<Longrightarrow>LENGTH('c) + LENGTH('b) = LENGTH('d)
+\<Longrightarrow> LENGTH('e) + LENGTH('d) = LENGTH('a)
+\<Longrightarrow> LENGTH('f) = LENGTH('a) - LENGTH('b)
+\<Longrightarrow> LENGTH('f) = LENGTH('c) + LENGTH('e)
+\<Longrightarrow> LENGTH('f) + LENGTH('b) = LENGTH('a)
+
+\<Longrightarrow> xs \<noteq> (ListVar []) \<Longrightarrow> ws \<noteq> (ListVar []) \<Longrightarrow> is_singleton_ListVar ys
+\<Longrightarrow>
+   (cvc_list_left xor xs
+     (cvc_list_right xor
+       (word_cat_helper_left 
+         ys
+         (word_cat z y ::'d ::len word)
+       ::'a::len word)
+       ws
+     ::'a word)
+   ::'a word)
+= 
+  (word_cat
+    ( xor
+      (smt_extract ( LENGTH('a) - 1) (LENGTH('b)) (cvc_list_both' xor xs ws ::'a::len word)::'f::len word)
+      (word_cat_helper_left ys (z::'c::len word)::'f::len word)
+    ::'f::len word)
+    (xor (smt_extract (LENGTH('b) - 1) (nat 0) (cvc_list_both' xor xs ws ::'a word)::'b::len word) y ::'b word)
+  ::'a word)
+   "
+  apply (cases xs)
+  apply (cases ws)
+  apply (cases ys)
+  apply simp
+  subgoal for xs' ws' ys'
+    apply (cases ys')
+     apply simp_all
+    subgoal for y1 ys1
+    proof-
+      assume  a0:
+        "LENGTH('e) + LENGTH('d) = LENGTH('a)"
+    "LENGTH('c) + LENGTH('e) = LENGTH('a) - LENGTH('b)"
+    "LENGTH('f) = LENGTH('a) - LENGTH('b)"
+    "LENGTH('a) - LENGTH('b) + LENGTH('b) = LENGTH('a)"
+    "xs' \<noteq> []"
+    "ws' \<noteq> []"
+    "ys1 = []"
+    "xs = ListVar xs'"
+    "ws = ListVar ws'"
+    "ys = ListVar [y1]"
+    "ys' = [y1]"
+      obtain t1 where t1_def: "t1 \<equiv>  (cvc_list_both' xor (ListVar xs') (ListVar ws'))"
+        by blast
+      obtain t2 where t2_def: "t2 \<equiv>  (word_cat y1 z::'f::len word)"
+        by blast
+
+
+      have "cvc_list_left xor (ListVar xs') (cvc_list_right xor (word_cat y1 (word_cat z y::'d::len word)) (ListVar ws')) =
+(xor (word_cat y1 (word_cat z y::'d::len word)) (cvc_list_both' xor (ListVar xs') (ListVar ws')) )"
+        by (metis (no_types, lifting) \<open>(ws'::'a::len word list) \<noteq> []\<close> \<open>(xs'::'a::len word list) \<noteq> []\<close> cvc_list_both_transfer' cvc_list_left_transfer cvc_list_right_transfer_2 fold_b helper3 helper4)
+      then have "cvc_list_left xor (ListVar xs') (cvc_list_right xor (word_cat y1 (word_cat z y::'d::len word)) (ListVar ws')) =
+(xor (word_cat y1 (word_cat z y::'d::len word)) t1 )"
+          using t1_def by simp
+ then have "cvc_list_left xor (ListVar xs') (cvc_list_right xor (word_cat y1 (word_cat z y::'d::len word)) (ListVar ws')) =
+(xor (word_cat (word_cat y1 z::'f::len word) y ::'a::len word) t1 )"
+   apply (subst word_cat_on_word_cat[symmetric,of y1 z y, where 'a='f and 'b='a and 'd='d])
+   using a0
+   apply (simp_all add: a0 word_size)
+   using a0(2) apply presburger
+   using a0(1) a0(2) a0(4) apply linarith
+   by (metis (no_types, lifting) a0(5) a0(6) cvc_list_both_transfer' cvc_list_left_transfer cvc_list_right_transfer_2 fold_b helper3 helper4 t1_def)
+    then have "cvc_list_left xor (ListVar xs') (cvc_list_right xor (word_cat y1 (word_cat z y::'d::len word)) (ListVar ws')) =
+(xor (word_cat (t2::'f::len word) y ::'a::len word) t1 )"
+      using t2_def by simp
+ then have "cvc_list_left xor (ListVar xs') (cvc_list_right xor (word_cat y1 (word_cat z y::'d::len word)) (ListVar ws')) =
+word_cat (xor (smt_extract (LENGTH('a::len) - (1::nat)) LENGTH('b::len) t1) t2) (xor (smt_extract (LENGTH('b::len) - (1::nat)) (nat (0::int)) t1) y)"
+   by (simp add: a0 rewrite_bv_xor_concat_pullup_lemma0[of t2 y t1])
+
+
+  then    show "cvc_list_left xor (ListVar xs') (cvc_list_right xor (word_cat y1 (word_cat z y::'d::len word)) (ListVar ws')) =
+    word_cat (xor (smt_extract (LENGTH('a) - Suc (0::nat)) LENGTH('b) (cvc_list_both' xor (ListVar xs') (ListVar ws'))) (word_cat y1 z)::'f::len word)
+     (xor (smt_extract (LENGTH('b) - Suc (0::nat)) (0::nat) (cvc_list_both' xor (ListVar xs') (ListVar ws'))) y)"
+
+    by (simp add: t1_def t2_def)
+qed
+  done
+  done
+
+
+(*    foldr neq (map bit_n xs')
+     (bit (xor (smt_extract n (0::nat) y) (foldr xor (map (smt_extract n (0::nat)) (butlast ws')) (smt_extract n (0::nat) (last ws')))) n)
+
+ =
+    foldr neq (map (bit_n \<circ> smt_extract (LENGTH('b) - Suc (0::nat)) (0::nat)) xs')
+     (foldr (\<lambda>(x::bool) y::bool. x = (\<not> y)) (map ((\<lambda>x::'b word. bit x n) \<circ> smt_extract (LENGTH('b) - Suc (0::nat)) (0::nat)) (butlast ws'))
+       (bit (xor (smt_extract (LENGTH('b) - Suc (0::nat)) (0::nat) (last ws')) y) n))*)
+
+
+
+
+
+
+
+
+
+
+
+
+
+
+
+
+
+
+
+(*
+lemma h1:
+  fixes xs::"('a::len word) cvc_ListVar"
+    and ws::"('a::len word) cvc_ListVar"
+    and y::"'b::len word"
+    and z::"'c::len word"
+    and ys::"('e::len word) cvc_ListVar"
+    and nxm1::"int" and ny::"int" and nym1::"int"
+  shows "NO_MATCH cvc_a (undefined xs ws y z ys nxm1 ny nym1)
+\<Longrightarrow> LENGTH('a) = LENGTH('b) + LENGTH('c)
+\<Longrightarrow> LENGTH('c) = nat nxm1 - nat ny + 1
+\<Longrightarrow> LENGTH('b) = nat nym1 + 1
+\<Longrightarrow> LENGTH('b) + LENGTH('c) = LENGTH('a)
+\<Longrightarrow> xs \<noteq> (ListVar []) \<Longrightarrow> ws \<noteq> (ListVar []) \<Longrightarrow> is_empty_ListVar ys
+\<Longrightarrow> nxm1 \<ge> 0 \<Longrightarrow> ny \<ge> 0 \<Longrightarrow> nym1 \<ge> 0
+\<Longrightarrow> n < LENGTH('c) \<Longrightarrow> n < LENGTH('a) \<Longrightarrow> n + nat ny < Suc (nat nxm1)
+\<Longrightarrow>
+   bit (cvc_list_left xor xs
+     (cvc_list_right xor
+      (word_cat z y ::'a ::len word)
+       ws
+     ::'a word)
+   ::'a word) n
+= 
+  bit (
+    ( xor
+      (smt_extract (nat nxm1) (nat ny) (cvc_list_both' xor xs ws ::'a::len word)::'c::len word)
+      (z::'c::len word)
+    ::'c::len word)
+    )  n
+   "
+  apply (cases xs)
+  apply (cases ws)
+  apply (cases ys)
+  apply simp
+  subgoal for xs' ws' ys'
+      unfolding cvc_list_left_transfer
+      apply (subst cvc_list_right_transfer_2)
+       apply simp_all
+      unfolding cvc_list_both_transfer'
+unfolding bit_xor_iff bit_smt_extract
+  proof-
+    assume a0:
+    "LENGTH('a) = Suc (Suc (nat nym1 + nat nxm1 - nat ny))"
+    "LENGTH('c) = Suc (nat nxm1 - nat ny)"
+    "LENGTH('b) = Suc (nat nym1)"
+    "xs' \<noteq> [] "
+    "ws' \<noteq> []"
+    "ys' = []"
+    "(0::int) \<le> nxm1"
+    "(0::int) \<le> ny"
+    "(0::int) \<le> nym1"
+    "n < Suc (nat nxm1 - nat ny)"
+    "n < Suc (Suc (nat nym1 + nat nxm1 - nat ny))"
+    "n + nat ny < Suc (nat nxm1)"
+    "xs = ListVar xs'"
+    "ws = ListVar ws'"
+    "ys = ListVar []"
+    have "((n + nat ny < Suc (nat nxm1) \<and> bit (foldr xor xs' (foldr xor (butlast ws') (last ws'))) (n + nat ny)) \<and>
+      n < LENGTH('c))
+      = ((n + nat ny < Suc (nat nxm1) \<and> bit (foldr xor xs' (foldr xor (butlast ws') (last ws'))) (n + nat ny)))"
+      using \<open>LENGTH('c::len) = Suc (nat (nxm1::int) - nat (ny::int))\<close> by linarith
+    then have h1: "((n + nat ny < Suc (nat nxm1) \<and> bit (foldr xor xs' (foldr xor (butlast ws') (last ws'))) (n + nat ny)) \<and>
+      n < LENGTH('c))
+      = ((bit (foldr xor xs' (foldr xor (butlast ws') (last ws'))) (n + nat ny)))"
+      using a0(12) by blast
+
+
+
+    show "bit (foldr xor xs' (xor (word_cat z y) (foldr xor (butlast ws') (last ws')))) n =
+    (((n + nat ny < Suc (nat nxm1) \<and> bit (foldr xor xs' (foldr xor (butlast ws') (last ws'))) (n + nat ny)) \<and>
+      n < LENGTH('c)) \<noteq>
+     bit z n)"
+      apply (simp only: h1)
+
+  
+  apply simp
+  apply (cases "n + nat ny < Suc (nat nxm1)")
+   apply simp
+       apply simp_all
+       unfolding cvc_list_left_transfer
+      apply (subst cvc_list_right_transfer_2)
+       apply simp_all
+       unfolding cvc_list_both_transfer'
+ unfolding bit_foldr_xor bit_xor_iff
+  unfolding bit_word_cat_iff
+  apply simp
+
+
+lemma [rewrite_bv_xor_concat_pullup]:
+  fixes xs::"('a::len word) cvc_ListVar"
+    and ws::"('a::len word) cvc_ListVar"
+    and y::"'b::len word"
+    and z::"'c::len word"
+    and ys::"('e::len word) cvc_ListVar"
+    and nxm1::"int" and ny::"int" and nym1::"int"
+  shows "NO_MATCH cvc_a (undefined xs ws y z ys nxm1 ny nym1)
+\<Longrightarrow> LENGTH('a) = LENGTH('b) + LENGTH('c)
+\<Longrightarrow> LENGTH('c) = nat nxm1 - nat ny + 1
+\<Longrightarrow> LENGTH('b) = nat nym1 + 1
+\<Longrightarrow> LENGTH('b) + LENGTH('c) = LENGTH('a)
+\<Longrightarrow> xs \<noteq> (ListVar []) \<Longrightarrow> ws \<noteq> (ListVar []) \<Longrightarrow> is_empty_ListVar ys
+\<Longrightarrow> nxm1 \<ge> 0 \<Longrightarrow> ny \<ge> 0 \<Longrightarrow> nym1 \<ge> 0
+\<Longrightarrow>
+   (cvc_list_left xor xs
+     (cvc_list_right xor
+      (word_cat z y ::'a ::len word)
+       ws
+     ::'a word)
+   ::'a word)
+= 
+  (word_cat
+    ( xor
+      (smt_extract (nat nxm1) (nat ny) (cvc_list_both' xor xs ws ::'a::len word)::'c::len word)
+      (z::'c::len word)
+    ::'c::len word)
+    (xor (smt_extract (nat nym1) (nat 0) (cvc_list_both' xor xs ws ::'a word)::'b::len word) y ::'b word)
+  ::'a word)
+   "
+  apply (cases xs)
+  apply (cases ws)
+  apply (cases ys)
+  apply simp
+  subgoal for xs' ws' ys'
+      unfolding cvc_list_left_transfer
+      apply (subst cvc_list_right_transfer_2)
+       apply simp_all
+      unfolding cvc_list_both_transfer'
+      apply (simp only: helper3 helper4)
+
+      unfolding word_cat_helper_left_def
+      apply (simp only: bang_eq)
+      apply (rule allI)
+      subgoal for n
+        apply (cases "n < LENGTH('b)")
+         apply (simp_all add: bit_word_cat_iff)
+        apply (simp_all add: bit_xor_iff bit_smt_extract)
+  sorry
+
+
+lemma 
+  fixes xs::"('a::len word) cvc_ListVar"
+    and ws::"('a::len word) cvc_ListVar"
+    and y::"'b::len word"
+    and z::"'c::len word"
+    and ys::"('e::len word) cvc_ListVar"
+    and nxm1::"int" and ny::"int" and nym1::"int"
+  shows "NO_MATCH cvc_a (undefined xs ws y z ys nxm1 ny nym1)
+\<Longrightarrow> LENGTH('d) = LENGTH('b) + LENGTH('c)
+\<Longrightarrow> LENGTH('a) = LENGTH('d) + LENGTH('e)
+\<Longrightarrow> LENGTH('f) = nat nxm1 - nat ny + 1
+\<Longrightarrow> LENGTH('e) + LENGTH('c) = LENGTH('f)
+\<Longrightarrow> LENGTH('b) = nat nym1 + 1
+\<Longrightarrow> LENGTH('b) + LENGTH('f) = LENGTH('a)
+\<Longrightarrow> xs \<noteq> (ListVar []) \<Longrightarrow> ws \<noteq> (ListVar []) \<Longrightarrow> is_singleton_ListVar ys
+\<Longrightarrow> nxm1 \<ge> 0 \<Longrightarrow> ny \<ge> 0 \<Longrightarrow> nym1 \<ge> 0
+\<Longrightarrow>
+   (cvc_list_left xor xs
+     (cvc_list_right xor
+       (word_cat_helper_left
+         ys
+         (word_cat z y ::'d ::len word)
+        ::'a word) ws
+     ::'a word)
+   ::'a word)
+= 
+  (word_cat
+    ( xor
+      (smt_extract (nat nxm1) (nat ny) (cvc_list_both' xor xs ws ::'a::len word)::'f::len word)
+      (word_cat_helper_left ys z::'f::len word)
+    ::'f::len word)
+    (xor (smt_extract (nat nym1) 0 (cvc_list_both' xor xs ws ::'a word)::'b::len word) y ::'b word)
+  ::'a word)
+   "
+  apply (cases xs)
+  apply (cases ws)
+  apply (cases ys)
+  apply simp
+  subgoal for xs' ws' ys'
+      unfolding cvc_list_left_transfer
+      apply (subst cvc_list_right_transfer_2)
+       apply simp_all
+      unfolding cvc_list_both_transfer'
+      apply (cases ys') 
+       apply simp_all
+      subgoal for ys'' ys_empty
+        apply (induction xs' arbitrary: xs)
+         apply simp
+        apply (induction ys' arbitrary: ys)
+         apply simp
+        apply simp
+
+
+      unfolding word_cat_helper_left_def
+       apply simp_all
+
+        sorry
+
+
+lemma
+ fixes xs::"('a::len word) cvc_ListVar"
+    and ws::"('a::len word) cvc_ListVar"
+    and y::"'b::len word"
+    and z::"'c::len word"
+    and ys::"('e::len word) cvc_ListVar"
+    and nxm1::"int" and ny::"int" and nym1::"int"
+  shows
+    "LENGTH('a) = LENGTH('d) + LENGTH('e)\<longrightarrow>
+    LENGTH('f) = Suc (nat nxm1 - nat ny) \<longrightarrow>
+    LENGTH('e) + LENGTH('c) = Suc (nat nxm1 - nat ny) \<longrightarrow>
+    LENGTH('b) = Suc (nat nym1) \<longrightarrow>
+    Suc (Suc (nat nym1 + (nat nxm1 - nat ny))) = LENGTH('d) + LENGTH('e) \<longrightarrow>
+    xs' \<noteq> [] \<longrightarrow>
+    ws' \<noteq> [] \<longrightarrow>
+    ys_empty = [] \<longrightarrow>
+    (0::int) \<le> nxm1 \<longrightarrow>
+    (0::int) \<le> ny \<longrightarrow>
+    (0::int) \<le> nym1 \<longrightarrow>
+    xs = ListVar xs' \<longrightarrow>
+    ws = ListVar ws' \<longrightarrow>
+    ys = ListVar [ys''] \<longrightarrow>
+    ys' = [ys''] \<longrightarrow>
+    foldr xor xs' (xor (word_cat ys'' (word_cat z y::'d::len word)) (foldr xor (butlast ws') (last ws'))) =
+    word_cat (xor (smt_extract (nat nxm1) (nat ny) (foldr xor xs' (foldr xor (butlast ws') (last ws')))) (word_cat ys'' z))
+     (xor (smt_extract (nat nym1) (0::nat) (foldr xor xs' (foldr xor (butlast ws') (last ws')))) y)"
+
+
+lemma
+  fixes xs::"('a::len word) cvc_ListVar"
+    and ws::"('a::len word) cvc_ListVar"
+    and y::"'b::len word"
+    and z::"'c::len word"
+    and ys::"(bool list) list"
+    and nxm1::"nat" and ny::"nat" and nym1::"nat"
+  shows "NO_MATCH cvc_a (undefined xs ws y z ys nxm1 ny nym1)
+\<Longrightarrow> length (concat ys) = LENGTH('e)
+\<Longrightarrow> LENGTH('d) = LENGTH('b) + LENGTH('c)
+\<Longrightarrow> LENGTH('a) = LENGTH('d) + LENGTH('e)
+\<Longrightarrow> LENGTH('f) = nxm1 - ny + 1
+\<Longrightarrow> LENGTH('e) + LENGTH('c) = LENGTH('f)
+\<Longrightarrow> LENGTH('b) = nym1 + 1
+\<Longrightarrow> LENGTH('b) + LENGTH('f) = LENGTH('a)
+\<Longrightarrow> xs \<noteq> (ListVar []) \<Longrightarrow> ws \<noteq> (ListVar []) 
+\<Longrightarrow>
+   (cvc_list_left xor xs
+     (cvc_list_right xor
+       (word_cat
+         (of_bl (concat ys)::'e::len word)
+         (word_cat z y ::'d ::len word)
+        ::'a word) ws
+     ::'a word)
+   ::'a word)
+= 
+  (word_cat
+    ( xor
+      (smt_extract nxm1 ny (cvc_list_both' xor xs ws ::'a::len word)::'f::len word)
+      (word_cat (of_bl (concat ys)::'e::len word) z::'f::len word)
+    ::'f::len word)
+    (xor (smt_extract nym1 0 (cvc_list_both' xor xs ws ::'a word)::'b::len word) y ::'b word)
+  ::'a word)
+   "
+  apply (cases xs)
+  apply (cases ws)
+  apply simp
+  subgoal for xs' ws'
+      unfolding cvc_list_left_transfer
+      apply (subst cvc_list_right_transfer_2)
+       apply simp_all
+      unfolding cvc_list_both_transfer'
+      apply (induction xs' arbitrary: xs)
+      apply simp_all
+      apply (induction ws' arbitrary: ws)
+       apply simp_all
+      apply (rule impI conjI)+
+      sorry
+    sorry
+*)
+
+lemma
+  assumes  "(1::int) = int (size (0::1 word))" 
+    and "(7::int) = int (size (27::8 word)) - (1::int)"
+    and "(0::int) = int (size (0::1 word)) - (1::int)"
+  shows "xor (27::8 word) (word_cat (smt_extract 6 0 (v0::8 word)::7 word) (0::1 word)::8 word) =
+        word_cat
+          (xor (smt_extract 7 1 (27::8 word)::7 word) (smt_extract 6 0 v0 :: 7 word) :: 7 word)
+          (xor (smt_extract 0 0 (27::8 word)::1 word) (0::1 word) :: 1 word) "
+  sorry
+
+
+(*
+(define-cond-rule bv-and-concat-pullup2
+  ((xs ?BitVec :list) (ws ?BitVec :list) (y ?BitVec)
+   (z ?BitVec) (ys ?BitVec :list)
+   (nxm1 Int) (ny Int) (nym1 Int))
+  (def
+    (s (@bvsize (bvand xs ws)))
+    (sy (@bvsize (concat y ys)))
+  )
+  (and (= ny sy) (= nxm1 (- s 1)) (= nym1 (- sy 1)))
+  (bvand xs (concat z y ys) ws)
+  (concat
+    (bvand (extract nxm1 ny (bvand xs ws)) z)
+    (bvand (extract nym1 0 (bvand xs ws)) (concat y ys))
+  ))
+*)
+
+(*
+(define-cond-rule bv-or-concat-pullup2
+  ((xs ?BitVec :list) (ws ?BitVec :list) (y ?BitVec)
+   (z ?BitVec) (ys ?BitVec :list)
+   (nxm1 Int) (ny Int) (nym1 Int))
+  (def
+    (s (@bvsize (bvor xs ws)))
+    (sy (@bvsize (concat y ys)))
+  )
+  (and (= ny sy) (= nxm1 (- s 1)) (= nym1 (- sy 1)))
+  (bvor xs (concat z y ys) ws)
+  (concat
+    (bvor (extract nxm1 ny (bvor xs ws)) z)
+    (bvor (extract nym1 0 (bvor xs ws)) (concat y ys))
+  ))
+*)
+
+
+(*
+(define-cond-rule bv-xor-concat-pullup2
+  ((xs ?BitVec :list) (ws ?BitVec :list) (y ?BitVec)
+   (z ?BitVec) (ys ?BitVec :list)
+   (nxm1 Int) (ny Int) (nym1 Int))
+  (def
+    (s (@bvsize (bvxor xs ws)))
+    (sy (@bvsize (concat y ys)))
+  )
+  (and (= ny sy) (= nxm1 (- s 1)) (= nym1 (- sy 1)))
+  (bvxor xs (concat z y ys) ws)
+  (concat
+    (bvxor (extract nxm1 ny (bvxor xs ws)) z)
+    (bvxor (extract nym1 0 (bvxor xs ws)) (concat y ys))
+  ))
+*)
+
+
+
+(*
+(define-cond-rule bv-and-concat-pullup3
+  ((xs ?BitVec :list) (ws ?BitVec :list) (y ?BitVec)
+   (z ?BitVec) (u ?BitVec)
+   (nxm1 Int) (nyu Int) (nyum1 Int) (nu Int) (num1 Int))
+  (def
+    (s (@bvsize (bvand xs ws)))
+    (su (@bvsize u))
+    (sy (@bvsize y))
+  )
+  (and (= nxm1 (- s 1)) (= nyu (+ sy su)) (= nyum1 (- (+ sy su) 1)) (= nu su) (= num1 (- su 1)))
+  (bvand xs (concat z y u) ws)
+  (concat
+    (bvand (extract nxm1 nyu (bvand xs ws)) z)
+    (bvand (extract nyum1 nu (bvand xs ws)) y)
+    (bvand (extract num1 0 (bvand xs ws)) u)
+  ))
+*)
+
+
+(*
+(define-cond-rule bv-or-concat-pullup3
+  ((xs ?BitVec :list) (ws ?BitVec :list) (y ?BitVec)
+   (z ?BitVec) (u ?BitVec)
+   (nxm1 Int) (nyu Int) (nyum1 Int) (nu Int) (num1 Int))
+  (def
+    (s (@bvsize (bvor xs ws)))
+    (su (@bvsize u))
+    (sy (@bvsize y))
+  )
+  (and (= nxm1 (- s 1)) (= nyu (+ sy su)) (= nyum1 (- (+ sy su) 1)) (= nu su) (= num1 (- su 1)))
+  (bvor xs (concat z y u) ws)
+  (concat
+    (bvor (extract nxm1 nyu (bvor xs ws)) z)
+    (bvor (extract nyum1 nu (bvor xs ws)) y)
+    (bvor (extract num1 0 (bvor xs ws)) u)
+  ))
+*)
+
+(*
+(define-cond-rule bv-xor-concat-pullup3
+  ((xs ?BitVec :list) (ws ?BitVec :list) (y ?BitVec)
+   (z ?BitVec) (u ?BitVec)
+   (nxm1 Int) (nyu Int) (nyum1 Int) (nu Int) (num1 Int))
+  (def
+    (s (@bvsize (bvxor xs ws)))
+    (su (@bvsize u))
+    (sy (@bvsize y))
+  )
+  (and (= nxm1 (- s 1)) (= nyu (+ sy su)) (= nyum1 (- (+ sy su) 1)) (= nu su) (= num1 (- su 1)))
+  (bvxor xs (concat z y u) ws)
+  (concat
+    (bvxor (extract nxm1 nyu (bvxor xs ws)) z)
+    (bvxor (extract nyum1 nu (bvxor xs ws)) y)
+    (bvxor (extract num1 0 (bvxor xs ws)) u)
+  ))
+*)
+
+
+(*
+(define-cond-rule bv-xor-duplicate ((x ?BitVec) (w Int))
+  (= w (@bvsize x))
+  (bvxor x x) 
+  (@bv 0 w))
+*)
+
+
+(*
+(define-cond-rule bv-xor-ones ((xs ?BitVec :list) (zs ?BitVec :list) (n Int) (w Int))
+  (= n (- (int.pow2 w) 1))
+  (bvxor xs (@bv n w) zs)
+  (bvnot (bvxor xs zs)))
+*)
+
+
+(*
+(define-rule bv-xor-not ((x ?BitVec) (y ?BitVec))
+  (bvxor (bvnot x) (bvnot y)) (bvxor x y))
+*)
+
+
+(*
+(define-rule bv-not-idemp ((x ?BitVec))
+  (bvnot (bvnot x)) x)
+*)
+
+
+(*
+(define-rule bv-ult-zero-1
+  ((x ?BitVec) (n Int))
+  (bvult (@bv 0 n) x)
+  (not (= x (@bv 0 n))))
+*)
+
+
+(*
+(define-rule bv-ult-zero-2
+  ((x ?BitVec) (n Int))
+  (bvult x (@bv 0 n))
+  false)
+*)
+
+
+(*
+(define-rule bv-ult-self ((x ?BitVec)) (bvult x x) false)
+*)
+
+
+(*
+(define-rule bv-lt-self ((x ?BitVec)) (bvslt x x) false)
+*)
+
+
+(*
+(define-rule bv-ule-self ((x ?BitVec)) (bvule x x) true)
+*)
+
+
+(*
+(define-rule bv-ule-zero
+  ((x ?BitVec) (n Int))
+  (bvule x (@bv 0 n))
+  (= x (@bv 0 n)))
+*)
+
+
+named_theorems rewrite_bv_ule_zero \<open>automatically_generated\<close>
+
+lemma [rewrite_bv_ule_zero]:
+  fixes x::"'a ::len word" and n::"int"
+  shows "NO_MATCH cvc_a (undefined x n) 
+    \<Longrightarrow> LENGTH('a) = n
+    \<Longrightarrow> (x \<le> 0) = (x = 0)"
+  by auto
+
+(*
+(define-rule bv-zero-ule
+  ((x ?BitVec) (n Int))
+  (bvule (@bv 0 n) x)
+  true)
+*)
+
+
+(*
+(define-rule bv-sle-self ((x ?BitVec)) (bvsle x x) true)
+*)
+
+
+
+(*
+(define-cond-rule bv-ule-max ((x ?BitVec) (n Int) (w Int))
+  (and (= w (@bvsize x)) (= n (- (int.pow2 (@bvsize x)) 1)))
+  (bvule x (@bv n w)) true)
+*)
+
+
+(*
+(define-rule bv-not-ult ((x ?BitVec) (y ?BitVec))
+  (not (bvult x y))
+  (bvule y x))
+*)
+
+
+
+(*
+(define-cond-rule bv-mult-pow2-1
+  ((xs ?BitVec :list) (ys ?BitVec :list) (z ?BitVec) (size Int) (n Int) (exponent Int) (u Int))
+  (def (e (int.log2 n)))
+  (and (int.ispow2 n) (= exponent e) (= u (- (- size e) 1)))
+  (bvmul xs z (@bv n size) ys)
+  (concat
+    (extract u 0 (bvmul xs z ys))
+    (@bv 0 exponent)))
+*)
+
+
+(*
+(define-cond-rule bv-mult-pow2-2
+  ((xs ?BitVec :list) (ys ?BitVec :list) (z ?BitVec) (size Int) (n Int) (exponent Int) (u Int))
+  (def (ns (- (int.pow2 size) n)) (e (int.log2 ns)))
+  (and (int.ispow2 ns) (= exponent e) (= u (- (- size e) 1)))
+  (bvmul xs z (@bv n size) ys)
+  (concat
+    (extract u 0 (bvneg (bvmul xs z ys)))
+    (@bv 0 exponent)))
+*)
+
+
+(*
+(define-cond-rule bv-mult-pow2-2b
+  ((z ?BitVec) (size Int) (n Int) (exponent Int) (u Int))
+  (def (ns (- (int.pow2 size) n)) (e (int.log2 ns)))
+  (and (int.ispow2 ns) (= exponent e) (= u (- (- size e) 1)))
+  (bvmul z (@bv n size))
+  (concat
+    (extract u 0 (bvneg z))
+    (@bv 0 exponent)))
+*)
+
+(*
+(define-cond-rule bv-extract-mult-leading-bit
+  (
+    (high Int) (low Int)
+    (x1i Int) (x1in Int) (x2 ?BitVec)
+    (y1i Int) (y1in Int) (y2 ?BitVec)
+    (w Int)
+  )
+  (def
+    (n (+ x1in (@bvsize x2)))
+    (x0n (ite (= x1i 0) x1in (- x1in (+ 1 (int.log2 x1i)))))
+    (y0n (ite (= y1i 0) y1in (- y1in (+ 1 (int.log2 y1i)))))
+  )
+  (and (> n 64) (<= (- (\* 2 n) (+ x0n y0n)) low) (= w (+ 1 (- high low))))
+  (extract high low (bvmul
+    (concat (@bv x1i x1in) x2)
+    (concat (@bv y1i y1in) y2)))
+  (@bv 0 w))
+*)
+
+
+
+(*
+(define-cond-rule bv-udiv-pow2-not-one
+  ((x ?BitVec) (v Int) (n Int) (power Int) (nm1 Int))
+  (and (int.ispow2 v) (> v 1) (= power (int.log2 v)) (= nm1 (- n 1)))
+  (bvudiv x (@bv v n))
+  (concat (@bv 0 power) (extract nm1 power x)))
+*)
+
+
+
+(*
+(define-rule bv-udiv-zero
+  ((x ?BitVec) (n Int))
+  (bvudiv x (@bv 0 n))
+  (bvnot (@bv 0 n)))
+*)
+
+
+(*
+(define-rule bv-udiv-one ((x ?BitVec) (n Int))
+  (bvudiv x (@bv 1 n))
+  x)
+*)
+
+
+(*
+(define-cond-rule bv-urem-pow2-not-one
+  ((x ?BitVec) (v Int) (n Int) (nmp Int) (pm1 Int))
+  (def (power (int.log2 v)))
+  (and (int.ispow2 v) (> v 1) (= nmp (- n power)) (= pm1 (- power 1)))
+  (bvurem x (@bv v n))
+  (concat (@bv 0 nmp) (extract pm1 0 x)))
+*)
+
+
+
+(*
+(define-rule bv-urem-one
+  ((x ?BitVec) (n Int))
+  (bvurem x (@bv 1 n))
+  (@bv 0 n))
+*)
+
+
+(*
+(define-cond-rule bv-urem-self
+  ((x ?BitVec) (w Int))
+  (= w (@bvsize x))
+  (bvurem x x)
+  (@bv 0 w))
+*)
+
+
+(*
+(define-rule bv-shl-zero
+  ((a ?BitVec) (n Int))
+  (bvshl (@bv 0 n) a)
+  (@bv 0 n))
+*)
+
+
+(*
+(define-rule bv-lshr-zero
+  ((a ?BitVec) (n Int))
+  (bvlshr (@bv 0 n) a)
+  (@bv 0 n))
+*)
+
+
+(*
+(define-rule bv-ashr-zero
+  ((a ?BitVec) (n Int))
+  (bvashr (@bv 0 n) a)
+  (@bv 0 n))
+*)
+
+named_theorems rewrite_bv_ashr_zero \<open>automatically_generated\<close>
+
+lemma [rewrite_bv_ashr_zero]:
+  fixes n::"int" and a::"'a ::len word"
+  shows "NO_MATCH cvc_a (undefined a n) 
+    \<Longrightarrow> signed_drop_bit (unat a) 0 = 0"
+  by auto
+
+(*
+(define-cond-rule bv-ugt-urem
+  ((y ?BitVec) (x ?BitVec) (w Int))
+  (= w (@bvsize y))
+  (bvugt (bvurem y x) x)
+  (and
+    (= x (@bv 0 w))
+    (bvugt y (@bv 0 w))
+  ))
+*)
+
+
+
+(*
+(define-rule bv-ult-one
+  ((x ?BitVec) (n Int))
+  (bvult x (@bv 1 n))
+  (= x (@bv 0 n)))
+*)
+
+
+(*
+(define-cond-rule bv-slt-zero
+  ((x ?BitVec) (n Int) (nm1 Int))
+  (= nm1 (- n 1))
+  (bvslt x (@bv 0 n))
+  (= (extract nm1 nm1 x) (@bv 1 1)))
+*)
+
+
+
+(*
+(define-cond-rule bv-merge-sign-extend-1
+  ((x ?BitVec) (i Int) (j Int) (k Int))
+  (= k (+ i j))
+  (sign_extend i (sign_extend j x))
+  (sign_extend k x)
+  )
+*)
+
+
+(*
+(define-cond-rule bv-merge-sign-extend-2
+  ((x ?BitVec) (i Int) (j Int) (k Int))
+  (and (> j 0) (= k (+ i j)))
+  (sign_extend i (zero_extend j x))
+  (zero_extend k x)
+  )
+*)
+
+
+(*
+(define-cond-rule bv-sign-extend-eq-const-1
+  ((x ?BitVec) (m Int) (c Int) (nm Int) (mp1 Int) (nm1 Int) (nmm1 Int))
+  (def
+    (n (@bvsize x))
+    (clo (extract nm1 0 (@bv c nm)))
+    ; Combines the sign bit c[n-1] and the high part
+    (chi (extract nmm1 nm1 (@bv c nm)))
+  )
+  (and (= mp1 (+ m 1)) (= nm1 (- n 1)) (= nmm1 (- nm 1)))
+  (= (sign_extend m x) (@bv c nm))
+  (and
+    (or (= chi (@bv 0 mp1)) (= chi (bvnot (@bv 0 mp1))))
+    (= x clo)))
+*)
+
+
+(*
+(define-cond-rule bv-sign-extend-eq-const-2
+  ((x ?BitVec) (m Int) (c Int) (nm Int) (mp1 Int) (nm1 Int) (nmm1 Int))
+  (def
+    (n (@bvsize x))
+    (clo (extract nm1 0 (@bv c nm)))
+    ; Combines the sign bit c[n-1] and the high part
+    (chi (extract nmm1 nm1 (@bv c nm)))
+  )
+  (and (= mp1 (+ m 1)) (= nm1 (- n 1)) (= nmm1 (- nm 1)))
+  (= (@bv c nm) (sign_extend m x))
+  (and
+    (or (= chi (@bv 0 mp1)) (= chi (bvnot (@bv 0 mp1))))
+    (= x clo)))
+*)
+
+
+(*
+(define-cond-rule bv-zero-extend-eq-const-1
+  ((x ?BitVec) (m Int) (c Int) (nm Int) (nm1 Int) (nmm1 Int))
+  (def
+    (n (@bvsize x))
+    (clo (extract nm1 0 (@bv c nm)))
+    (chi (extract nmm1 nm1 (@bv c nm)))
+  )
+  (and (= nm1 (- n 1)) (= nmm1 (- nm 1)))
+  (= (zero_extend m x) (@bv c nm))
+  (and
+    (= chi (@bv 0 m))
+    (= x clo)))
+*)
+
+
+(*
+(define-cond-rule bv-zero-extend-eq-const-2
+  ((x ?BitVec) (m Int) (c Int) (nm Int) (nm1 Int) (nmm1 Int))
+  (def
+    (n (@bvsize x))
+    (clo (extract nm1 0 (@bv c nm)))
+    (chi (extract nmm1 nm1 (@bv c nm)))
+  )
+  (and (= nm1 (- n 1)) (= nmm1 (- nm 1)))
+  (= (@bv c nm) (zero_extend m x))
+  (and
+    (= chi (@bv 0 m))
+    (= x clo)))
+*)
+
+
+
+(*
+(define-cond-rule bv-zero-extend-ult-const-1
+  ((x ?BitVec) (m Int) (c Int) (nm Int) (nm1 Int))
+  (def
+    (n (@bvsize x))
+    (clo (extract nm1 0 (@bv c nm)))
+  )
+  (and (= nm1 (- n 1)) (= (@bv c nm) (zero_extend m clo)))
+  (bvult (zero_extend m x) (@bv c nm))
+  (bvult x clo))
+*)
+
+
+
+(*
+(define-cond-rule bv-zero-extend-ult-const-2
+  ((x ?BitVec) (m Int) (c Int) (nm Int) (nm1 Int))
+  (def
+    (n (@bvsize x))
+    (clo (extract nm1 0 (@bv c nm)))
+  )
+  (and (= nm1 (- n 1)) (= (@bv c nm) (zero_extend m clo)))
+  (bvult (@bv c nm) (zero_extend m x))
+  (bvult clo x))
+*)
+
+
+
+(*
+(define-cond-rule bv-sign-extend-ult-const-1
+  ((x ?BitVec) (m Int) (c Int) (nm Int) (nm1 Int))
+  (def
+    (n (@bvsize x))
+    (clo (extract nm1 0 (@bv c nm)))
+    (a (bvshl (@bv 1 nm) (@bv (- n 1) nm))) ; 1 << (n-1)
+    (b (bvshl (bvnot (@bv 0 nm)) (@bv (- n 1) nm))) ; ~0 << (n-1)
+  )
+  (and (or (bvule (@bv c nm) a) (bvuge (@bv c nm) b)) (= nm1 (- n 1)))
+  (bvult (sign_extend m x) (@bv c nm))
+  (bvult x clo))
+*)
+
+
+(*
+(define-cond-rule bv-sign-extend-ult-const-2
+  ((x ?BitVec) (m Int) (c Int) (nm Int) (nm1 Int))
+  (def
+    (n (@bvsize x))
+    (a (bvshl (@bv 1 nm) (@bv (- n 1) nm))) ; 1 << (n-1)
+    (b (bvshl (bvnot (@bv 0 nm)) (@bv (- n 1) nm))) ; ~0 << (n-1)
+  )
+  (and (bvult a (@bv c nm)) (bvule (@bv c nm) b) (= nm1 (- n 1)))
+  (bvult (sign_extend m x) (@bv c nm))
+  (= (extract nm1 nm1 x) (@bv 0 1)))
+*)
+
+
+(*
+(define-cond-rule bv-sign-extend-ult-const-3
+  ((x ?BitVec) (m Int) (c Int) (nm Int) (nm1 Int))
+  (def
+    (n (@bvsize x))
+    (clo (extract nm1 0 (@bv c nm)))
+    (a (bvshl (@bv 1 nm) (@bv (- n 1) nm))) ; 1 << (n-1)
+    (b (bvshl (bvnot (@bv 0 nm)) (@bv (- n 1) nm))) ; ~0 << (n-1)
+  )
+  (and (or (bvult (@bv c nm) a) (bvuge (@bv c nm) (bvnot a))) (= nm1 (- n 1)))
+  (bvult (@bv c nm) (sign_extend m x))
+  (bvult clo x))
+*)
+
+
+
+(*
+(define-cond-rule bv-sign-extend-ult-const-4
+  ((x ?BitVec) (m Int) (c Int) (nm Int) (nm1 Int))
+  (def
+    (n (@bvsize x))
+    (a (bvshl (@bv 1 nm) (@bv (- n 1) nm))) ; 1 << (n-1)
+    (b (bvshl (bvnot (@bv 0 nm)) (@bv (- n 1) nm))) ; ~0 << (n-1)
+  )
+  (and (bvule (bvnot b) (@bv c nm)) (bvule (@bv c nm) (bvnot a)) (= nm1 (- n 1)))
+  (bvult (@bv c nm) (sign_extend m x))
+  (= (extract nm1 nm1 x) (@bv 1 1)))
+*)
+
+
+
+
+
+
+end
